work on Hnf

proof/Hnf.v
@@ -17,12 +17,11 @@ Implicit Types A B M N T t u v : term.
 
 Definition snterm := { x : term | sn x }.
 
+Require Import Coq.subtac.Subtac.
+Require Import Coq.subtac.FunctionalExtensionality.
+
 Program Definition sn_ord : snterm -> snterm -> Prop := 
   fun x y => ord_norm x y.
-
-Require Import ProofIrrelevance.
-
-Scheme acc_dep := Induction for Acc Sort Prop.
 
 Lemma redn_sn_wf : well_founded sn_ord.
 Proof.
@@ -35,52 +34,84 @@ Proof.
   intros.
   destruct y ; simpl in *.
   apply (H0 x0 H1 s).
-Qed.
+Defined.
 
-Unset Printing All.
-Program Fixpoint hnf (x : snterm) { wf x sn_ord } :  { y : term | red x y } :=
+(*
+Require Import Recdef.
+
+Function hnf (x : term) { wf ord_norm x } : term :=
   match x with
-  | App x y => 
-    let nf := hnf x in
-    match nf with
-    | Abs T v => hnf (subst y v)
-    | h => App h y
-    end
-  | _ => x
+    | App x y => 
+      match x with
+        | Abs T v => hnf (subst y v)
+        | h => App h y
+        end  
+    | _ => x
+  end.
+intros.
+constructor.
+right.
+red.
+auto with coc.
+unfold well_founded ; intros.
+*)
+
+Program Fixpoint hnf (x : snterm) {wf x sn_ord} :  { y : term | red x y } :=
+  match x with
+    | App x y => 
+      let nf := hnf x in
+        match nf with
+          | Abs T v => hnf (subst y v)
+          | h => App h y
+        end  
+    | Pi1 x =>
+      let nf := hnf x in
+      match nf with
+        | Pair T l r => hnf l          
+        | h => Pi1 h
+      end
+    | Pi2 x => 
+      let nf := hnf x in
+      match nf with
+        | Pair T l r => hnf r
+        | h => Pi2 h
+      end
+    | _ => x
   end.
 
-
 Solve Obligations using simpl ; intros ; rewrite <- H ; auto with coc.
+Obligations.
 
-Obligation 1.
-  intros.
-  destruct x ; simpl in * ; auto.
-  apply subterm_sn with x ; auto.
-  rewrite <- H ; auto with coc.
+Program Lemma sn_proj_subterm_sn : forall x : snterm, forall y : term, y = x -> forall z, subterm z y -> sn z.
+Proof.
+  intros ; destruct x ; simpl in *.
+  subst x ; apply subterm_sn with y ; auto.
 Qed.
+
+Solve Obligations using subtac_simpl ;  eapply sn_proj_subterm_sn ; eauto with coc subtac.
+Require Import ZArith.
 
 Obligation 2.
   intros.
+  clear hnf.
   unfold sn_ord ; simpl.
   constructor.
   constructor.
   destruct x ; simpl in * ; auto with coc.
   rewrite <- H ; auto with coc.
 Qed.
-Require Import Coq.subtac.Utils.
 
-Obligation 3.
+Next Obligation.
   intros.
   destruct_call hnf.
   simpl in *.
   destruct x ; simpl in *.
-  apply sn_red_sn with (App x0 y).
-  subst x ; auto.
-  apply trans_red_red with (App x1 y) ; auto with coc.
-  subst x1 ; auto with coc.
+  subst x x1.
+  apply sn_red_sn with (App x0 y) ; auto with coc.
+  apply trans_red_red with (App (Abs T v) y) ; auto with coc.
 Qed.
 
-Obligation 4.
+Next Obligation.
   intros.
   unfold sn_ord.
   destruct x ; simpl in *.
@@ -108,6 +139,229 @@ Qed.
 
 Obligation 8.
   intros.
+  unfold sn_ord ; simpl.
+  constructor.
+  constructor.
+  destruct x ; simpl in * ; auto with coc.
+  rewrite <- H ; auto with coc.
+Qed.
+
+Obligation 9 of hnf. 
+  intros.
+  destruct_call hnf.
+  simpl in *.
+  destruct x ; simpl in *.
+  clear hnf.
+  subst x x1.
+  apply sn_red_sn with (Pi1 x0) ; auto with coc.
+  apply trans_red_red with (Pi1 (Pair T l r)) ; auto with coc.
+Qed.
+
+Obligation 10.
+  intros.
+  unfold sn_ord.
+  destruct x ; simpl in *.
+  destruct_call hnf ; simpl in *.
+  subst x x1.
+  apply red_red1_ord_norm with (Pi1 (Pair T l r)) ; auto with coc.
+Qed.
+
+Obligation 11.
+  intros.
+  destruct_call hnf ; simpl in *.
+  destruct_call hnf ; simpl in *.
+  destruct x ; simpl in *.
+  subst x x2.
+  apply trans_red_red with l ; auto.
+  apply trans_red_red with (Pi1 (Pair T l r)) ; auto with coc.
+Qed.
+
+Obligation 12.
+  intros.
+  destruct x ; destruct_call hnf ; simpl in *.
+  subst x x1.
+  auto with coc.
+Qed.
+
+Obligation 14.
+  intros.
+  unfold sn_ord ; simpl.
+  constructor.
+  constructor.
+  destruct x ; simpl in * ; auto with coc.
+  rewrite <- H ; auto with coc.
+Qed.
+
+Obligation 15 of hnf. 
+  intros.
+  destruct_call hnf.
+  simpl in *.
+  destruct x ; simpl in *.
+  subst x x1.
+  apply sn_red_sn with (Pi2 x0) ; auto with coc.
+  apply trans_red_red with (Pi2 (Pair T l r)) ; auto with coc.
+Qed.
+
+Obligation 16.
+  intros.
+  unfold sn_ord.
+  destruct x ; simpl in *.
+  destruct_call hnf ; simpl in *.
+  subst x x1.
+  apply red_red1_ord_norm with (Pi2 (Pair T l r)) ; auto with coc.
+Qed.
+
+Obligation 17.
+  intros.
+  destruct_call hnf ; simpl in *.
+  destruct_call hnf ; simpl in *.
+  destruct x ; simpl in *.
+  subst x x2.
+  apply trans_red_red with r ; auto.
+  apply trans_red_red with (Pi2 (Pair T l r)) ; auto with coc.
+Qed.
+
+Obligation 18.
+  intros.
+  destruct x ; destruct_call hnf ; simpl in *.
+  subst x x1.
+  auto with coc.
+Qed.
+
+Obligation 20.
+  intros.
   apply redn_sn_wf.  
+Defined.
+
+Inductive hnf_graph : term -> term -> Prop :=
+| hnf_srt : forall s, hnf_graph (Srt s) (Srt s)
+| hnf_ref : forall n, hnf_graph (Ref n) (Ref n)
+| hnf_abs : forall A M, hnf_graph (Abs A M) (Abs A M)
+| hnf_beta : forall u T e, hnf_graph u (Abs T e) -> forall v hs, hnf_graph (subst v e) hs ->
+  hnf_graph (App u v) hs
+| hnf_app : forall u u', hnf_graph u u' -> (forall T e, u' <> Abs T e) -> forall v, hnf_graph (App u v) (App u' v)
+| hnf_pair :
+  forall T u v, hnf_graph (Pair T u v) (Pair T u v)
+| hnf_prod :
+  forall A B, hnf_graph (Prod A B) (Prod A B) 
+| hnf_sum :
+  forall A B, hnf_graph (Sum A B) (Sum A B)
+| hnf_subset :
+  forall A B, hnf_graph (Subset A B) (Subset A B)
+
+| hnf_proj1 : forall p T l r, hnf_graph p (Pair T l r) -> forall l', hnf_graph l l' -> hnf_graph (Pi1 p) l'
+| hnf_pi1 : forall p p', hnf_graph p p' -> (forall T l r, p' <> Pair T l r) -> hnf_graph (Pi1 p) (Pi1 p')
+
+| hnf_proj2 : forall p T l r, hnf_graph p (Pair T l r) -> forall r', hnf_graph r r' -> hnf_graph (Pi2 p) r'
+| hnf_pi2 : forall p p', hnf_graph p p' -> (forall T l r, p' <> Pair T l r) -> hnf_graph (Pi2 p) (Pi2 p').
+
+Program Definition hnf' (x : snterm) : term := hnf x.
+
+(*Goal let x := 1 in x = 0.
+Proof.
+  match goal with
+    | |- ?T =>
+      match T with
+        let x? := ?d in ?b => let x := fresh "x" in set (x := d)
+      end
+  end.
+*)
+
+Definition is_elim (x : term) : Prop := 
+  match x with
+    | App x y => True
+    | Pi1 _ => True
+    | Pi2 _ => True
+    | _ => False
+  end.
+
+Program Lemma not_elim_hnf : forall t : snterm, ~(is_elim t) -> (`t) = hnf t.
+Proof.
+  intros.
+  unfold hnf ; rewrite fix_sub_eq_ext.
+  induction t.
+  destruct x ; simpl ; auto ; simpl in H ; elim H ; auto.
+Qed.  
+
+Program Lemma hnf_graph_hnf : forall t : snterm, forall t' : term, hnf' t = t' -> hnf_graph t t'.
+Proof.
+  intros.
+  induction t.
+  unfold hnf' in H.
+  simpl.
+  rewrite <- H.
+  clear H.
+  unfold hnf.
+  rewrite fix_sub_eq_ext.
+  destruct x ; try (solve [(lazy beta iota delta [proj1_sig] ; lazy zeta iota beta ; try constructor)]).
+  
+  lazy beta iota delta [proj1_sig].
+  destruct x1 ; try (solve [(lazy beta iota delta [proj1_sig] ; lazy zeta iota beta ; try constructor)]).
+  
+  
+  
+
+simpl in H. 
+
+Lemma hnf_graph_total : forall t, sn t -> exists t', hnf_graph t t'.
+Proof.
+  intros t sn.
+  elimtype (Acc ord_norm t).
+  intros.
+  induction x ; try solve [(eapply ex_intro ; constructor)] ; destruct_exists.
+  
+  assert(ord_norm x1 (App x1 x2)).
+  constructor ; constructor ; auto with coc.
+  pose (H0 _ H1).
+  destruct_exists.
+  
+  set (x1' := x).
+  destruct x ; try solve [(exists (App x1' x2) ; apply hnf_app ; simpl ; intros ; auto with coc ; try (red ; intros ; discriminate))].
+  simpl in *.
+  clear x1'.
+  assert(ord_norm (subst x2 x4) (App x1 x2)).
+  unfold ord_norm.
+  apply t_trans with (App (Abs x3 x4) x2) ; constructor ; right ; unfold transp ; auto with coc.
+  
+  
+  
+  
+  
+  exists (
+  
+  
+  
+
+
+
+Program Definition hnf_prod_t := forall U V, sn (Prod U V) -> hnf (Prod U V) = Prod U V.
+Solve Obligations using simpl ; auto with coc.
+
+Lemma hnf_prod : hnf_prod_t.
+Proof.
+  red ; intros.
+  unfold hnf ; rewrite fix_sub_eq_ext ; simpl.
+  auto with coc subtac.
+Qed.
+
+
+Program Lemma hnf_sum : forall t : snterm, forall U V, Sum U V = t -> hnf' t = t.
+Proof.
+  intros.
+  unfold hnf' ; destruct t ; subtac_simpl.
+  simpl.
+  subst x.
+  unfold hnf ; rewrite fix_sub_eq_ext ; simpl.
+  auto with coc subtac.
+Qed.
+
+Program Lemma hnf_subset : forall t : snterm, forall U V, Subset U V = t -> hnf' t = t.
+Proof.
+  intros.
+  unfold hnf' ; destruct t ; subtac_simpl.
+  simpl.
+  subst x.
+  unfold hnf ; rewrite fix_sub_eq_ext ; simpl.
+  auto with coc subtac.
 Qed.
 
